add cost in library + br93 and hashed_elgamal_generic

examples/br93.ec
@@ -1,8 +1,8 @@
 (* -------------------------------------------------------------------- *)
 require import AllCore List FSet SmtMap.
 require import Distr DBool.
-require (*--*) BitWord OW ROM.
-
+require (*--*) BitWord OW ROM PKE_CPA CHoareTactic.
+(*---*) import StdBigop.Bigint BIA.
 (* ---------------- Sane Default Behaviours --------------------------- *)
 pragma -oldip.
 pragma +implicits.
@@ -37,6 +37,12 @@ lemma dptxt_uni: is_uniform dptxt by have [#]:= dptxt_llfuuni.
 lemma dptxt_fu: is_full dptxt by have [#]:= dptxt_llfuuni.
 lemma dptxt_funi: is_funiform dptxt
 by exact/(is_full_funiform dptxt_fu dptxt_uni).
+hint exact random : dptxt_ll dptxt_fu dptxt_funi.
+
+(* Complexity of sampling in dptxt *)
+op cdptxt : int.
+schema cost_dptxt `{P} : cost [P: dptxt] = cdptxt.
+hint simplify cost_dptxt.
 
 (* A set `rand` of nonces, equipped with                                *)
 (*                              a lossless, uniform distribution drand; *)
@@ -45,6 +51,16 @@ op drand: { rand distr |    is_lossless drand
                          /\ is_uniform drand } as drand_lluni.
 lemma drand_ll: is_lossless drand by exact/(andWl _ drand_lluni).
 lemma drand_uni: is_uniform drand by exact/(andWr _ drand_lluni).
+hint exact random : drand_ll drand_uni.
+
+(* Complexity of testing equality on rand *)
+op ceqrand : int.
+schema cost_eqrand `{P} {r1 r2:rand} : cost[P: r1 = r2] = cost[P:r1] + cost[P:r2] + ceqrand.
+hint simplify cost_eqrand.
+
+schema cost_witness_rand `{P} : cost [P: witness<:rand>] = 0. 
+hint simplify cost_witness_rand.
+
 
 (* A set `ctxt` of ciphertexts defined as                               *)
 (*                          the cartesian product of `rand` and `ptxt`; *)
@@ -68,6 +84,11 @@ lemma fI pk x y: (exists sk, (pk,sk) \in dkeys) =>
   f pk x = f pk y => x = y.
 proof. by move=> [sk] + fx_eq_fy - /fK ^ /(_ x) <- /(_ y) <-; congr. qed.
 
+(* Complexity of f *)
+op cf : int.
+schema cost_f `{P} {pk:pkey, r:rand} : cost [P: f pk r] = cost[P:pk] + cost[P:r] + cf.
+hint simplify cost_f.
+
 (* A random oracle from `rand` to `ptxt`, modelling a hash function H;  *)
 (* (we simply instantiate the generic theory of Random Oracles with     *)
 (*    the types and output distribution declared above, discharging all *)
@@ -77,18 +98,35 @@ clone import ROM.Lazy as H with
   type to    <- ptxt,
   op dsample <- fun _ => dptxt
 proof *.
-import Types.
+
+clone import FMapCost as FMC with
+  type from  <- rand.
+
+module type HASH = {
+  proc init(): unit
+  proc hash(x:rand): ptxt
+}.
+
+(* Specializing and merging the hash function *)
+
+module Hash = {
+  var qs : rand list
+  proc init(): unit = { RO.init(); qs <- []; }
+  proc o(x:rand): ptxt = { var y; qs <- x::qs; y <@ RO.o(x); return y; }
+  proc hash = RO.o
+}.
 
 (* We can define the Bellare-Rogaway 93 PKE Scheme.                     *)
 (* BR93 is a module that, given access to an oracle H from type         *)
 (*   `from` to type `rand` (see `print Oracle.`), implements procedures *)
 (*   `keygen`, `enc` and `dec` as follows described below.              *)
-module BR93 (H:Oracle) = {
+module BR93 (H:HASH) = {
   (* `keygen` simply samples a key pair in `dkeys` *)
-  proc keygen() = {
+  proc kg() = {
     var kp;
 
     kp <$ dkeys;
+    H.init();
     return kp;
   }
 
@@ -100,7 +138,7 @@ module BR93 (H:Oracle) = {
     var r, h;
 
     r <$ drand;
-    h <@ H.o(r);
+    h <@ H.hash(r);
     return (f pk r,h +^ m);
   }
 
@@ -114,40 +152,44 @@ module BR93 (H:Oracle) = {
 
     (r,m) <- c;
     r     <- fi sk r;
-    h     <- H.o(r);
+    h     <- H.hash(r);
     return h +^ m;
   }
 }.
 
+(* We instanciate the CPA game with the corresponding type *)
+clone import PKE_CPA as PKE with
+  type pkey <- pkey,
+  type skey <- skey,
+  type ptxt <- ptxt,
+  type ctxt <- ctxt.
+
 (* We can quickly prove it correct as a sanity check.                 *)
-section Correctness.
-local module Correctness = {
+module Correctness = {
   proc main(m) = {
     var pk, sk, c, m';
 
-    (pk,sk) <@ BR93(RO).keygen();
-    c       <@ BR93(RO).enc(pk,m);
-    m'      <@ BR93(RO).dec(sk,c);
+    (pk,sk) <@ BR93(Hash).kg();
+    c       <@ BR93(Hash).enc(pk,m);
+    m'      <@ BR93(Hash).dec(sk,c);
     return (m = m');
   }
 }.
 
-local lemma BR93_correct &m m: Pr[Correctness.main(m) @ &m: res] = 1%r.
+lemma BR93_correct &m m: Pr[Correctness.main(m) @ &m: res] = 1%r.
 proof.
 byphoare=> //; conseq (: _ ==> true) (: _ ==> res)=> //.
 + proc; inline *.
-  rcondf 17.
-  + auto=> /> &hr [pk sk] kp_in_dkeys r _ y _ /=.
+  rcondf 19.
+  + auto=> /> [pk sk] kp_in_dkeys r _ y _ /=.
     rewrite fK //; split=> [_ _ _|-> //].
     by rewrite mem_set.
   auto=> /> &hr [pk sk] kp_in_dkeys r _ y _ /=.
   rewrite fK //; split=> [_ y' _|].
   + by rewrite get_set_sameE -addA addKp.
-  rewrite domE; case: (RO.m{hr}.[r])=> [|p] //= _ _.
-  by rewrite -addA addKp.
+  + by rewrite mem_empty.
 by proc; inline *; auto=> />; rewrite dkeys_ll drand_ll dptxt_ll.
 qed.
-end section Correctness.
 
 (* However, what we are really interested in is proving that it is      *)
 (* IND-CPA secure if `f` is a one-way trapdoor permutation.             *)
@@ -168,62 +210,25 @@ realize challenge_ll by move=> _ _; exact/drand_ll.
 realize challenge_uni by move=> _ _; exact/drand_uni.
 realize finvof by move=> pk sk x /fK ->.
 
-(* But we can't do it (yet) for IND-CPA because of the random oracle    *)
-(*             Instead, we define CPA for BR93 with that particular RO. *)
 module type Adv (ARO: ARO)  = {
-  proc a1(p:pkey): (ptxt * ptxt)
-  proc a2(c:ctxt): bool
-}.
-
-(* We need to log the random oracle queries made to the adversary       *)
-(*                               in order to express the final theorem. *)
-module Log (H:Oracle) = {
-  var qs: rand list
-
-  proc init() = {
-    qs <- [];
-          H.init();
-  }
-
-  proc o(x) = {
-    var r;
-
-    qs <- x::qs;
-    r  <@ H.o(x);
-    return r;
-  }
-}.
-
-module BR93_CPA(A:Adv) = {
-  proc main(): bool = {
-    var pk, sk, m0, m1, c, b, b';
-
-                Log(RO).init();
-    (pk,sk)  <@ BR93(RO).keygen();
-    (m0,m1)  <@ A(Log(RO)).a1(pk);
-    b        <$ {0,1};
-    c        <@ BR93(RO).enc(pk,b?m0:m1);
-    b'       <@ A(Log(RO)).a2(c);
-    return b' = b;
-  }
+  proc choose(p:pkey): (ptxt * ptxt)
+  proc guess(c:ctxt): bool
 }.
 
 (* We want to prove the following:                                      *)
 (*   forall (valid) CPA adversary A which makes at most q queries to H, *)
 (*     there exists a OW adversary I such that                          *)
-(*          `|Pr[BR_CPA(A): res] - 1/2| <= Pr[OW_f(I): res]             *)
+(*          `|Pr[CPA(BR, A): res] - 1/2| <= Pr[OW_f(I): res]             *)
 (* We construct I as follows, using A.a1 and A.a2 as black boxes        *)
 module I(A:Adv): Inverter = {
-  var x:rand
-
   proc invert(pk:pkey,y:rand): rand = {
-    var m0, m1, h, b;
+    var m0, m1, h, b, x;
 
-               Log(RO).init();
-    (m0,m1) <@ A(Log(RO)).a1(pk);
+               Hash.init();
+    (m0,m1) <@ A(Hash).choose(pk);
     h       <$ dptxt;
-    b       <@ A(Log(RO)).a2(y,h);
-    x       <- nth witness Log.qs (find (fun p => f pk p = y) Log.qs);
+    b       <@ A(Hash).guess(y,h);
+    x       <- nth witness Hash.qs (find (fun p => f pk p = y) Hash.qs);
 
     return x;
   }
@@ -232,10 +237,9 @@ module I(A:Adv): Inverter = {
 (* We now prove the result using a sequence of games                    *)
 section.
 (* All lemmas in this section hold for all (valid) CPA adversary A      *)
-declare module A : Adv { -RO, -Log }.
+declare module A : Adv { -Hash }.
 
-axiom A_a1_ll (O <: ARO {-A}): islossless O.o => islossless A(O).a1.
-axiom A_a2_ll (O <: ARO {-A}): islossless O.o => islossless A(O).a2.
+axiom A_guess_ll (O <: ARO {-A}): islossless O.o => islossless A(O).guess.
 
 (* Step 1: replace RO call with random sampling                         *)
 local module Game1 = {
@@ -243,74 +247,40 @@ local module Game1 = {
 
   proc main() = {
     var pk, sk, m0, m1, b, h, c, b';
-                Log(RO).init();
+                Hash.init();
     (pk,sk)  <$ dkeys;
-    (m0,m1)  <@ A(Log(RO)).a1(pk);
+    (m0,m1)  <@ A(Hash).choose(pk);
     b        <$ {0,1};
 
     r        <$ drand;
     h        <$ dptxt;
-    c        <- ((f pk r),h +^ (b?m0:m1));
+    c        <- ((f pk r),h +^ (b?m1:m0));
 
-    b'       <@ A(Log(RO)).a2(c);
+    b'       <@ A(Hash).guess(c);
     return b' = b;
   }
 }.
 
 local lemma pr_Game0_Game1 &m:
-     Pr[BR93_CPA(A).main() @ &m: res]
+     Pr[CPA(BR93(Hash), A(Hash)).main() @ &m: res]
   <=   Pr[Game1.main() @ &m: res]
-     + Pr[Game1.main() @ &m: Game1.r \in Log.qs].
+     + Pr[Game1.main() @ &m: Game1.r \in Hash.qs].
 proof.
 byequiv=> //; proc.
-inline BR93(RO).enc BR93(RO).keygen.
+inline BR93(Hash).enc BR93(Hash).kg.
 (* Until the replaced RO call, the two games are in sync.               *)
 (*        In addition, the log's contents coincide with the RO queries. *)
-seq  8  5: (   ={glob A, glob RO, glob Log, pk, sk, b}
-            /\ pk0{1} = pk{2}
-            /\ m{1} = (b?m0:m1){2}
-            /\ r{1} = Game1.r{2}
-            /\ (forall x, x \in Log.qs{1} <=> x \in RO.m{1})).
-+ auto; call (:   ={glob Log, glob RO}
-               /\ (forall x, x \in Log.qs{1} <=> x \in RO.m{1})).
-  + proc; inline RO.o.
-    by auto=> /> &2 log_is_dom y _; smt(@SmtMap).
-  by inline *; auto=> /> _ _ x; rewrite mem_empty.
-(* We now deal with everything that happens after the programs differ: *)
-(*   - until r gets queried to the random oracle by the adversary      *)
-(*     (and if it wasn't already queried by a1), we guarantee that the *)
-(*     random oracles agree except on r                                *)
-(*   - if the adversary queries r to the random oracle (or if it has   *)
-(*     already done so in a1), we give up                              *)
-(* Because we reason up to bad, we need to prove that bad is stable    *)
-(* and that the adversary and its oracles are lossless                 *)
-call (_: Game1.r \in Log.qs,
+call (_: Game1.r \in Hash.qs,
+         (forall x, x \in Hash.qs{2} = x \in RO.m{2}) /\
          eq_except (pred1 Game1.r{2}) RO.m{1} RO.m{2}).
-+ exact/A_a2_ll.
-+ proc; inline RO.o.
-  auto=> /> &1 &2 _ m1_eqe_m2 yL y_in_dptxt; split.
-  + move=> x_notin_m; split.
-    + by rewrite !get_set_sameE eq_except_set_eq.
-    move: m1_eqe_m2 x_notin_m=> + + + r_neq_x.
-    by rewrite eq_exceptP pred1E !domE=> /(_ x{2} r_neq_x) ->.
-  move=> x_in_m; split.
-  + move: m1_eqe_m2 x_in_m=> + + + r_neq_x.
-    by rewrite eq_exceptP pred1E !domE=> /(_ x{2} r_neq_x) ->.
-  by move: m1_eqe_m2=> + _ r_neq_x- /eq_exceptP /(_ x{2}); rewrite pred1E=> /(_ r_neq_x) ->.
-+ by move=> &2 _; proc; call (RO_o_ll dptxt_ll); auto.
-+ move=> _ /=; proc; inline *.
-  conseq (: true ==> true: =1%r) (: Game1.r \in Log.qs ==> Game1.r \in Log.qs)=> //=.
-  + by auto=> />.
-  by auto=> />; exact/dptxt_ll.
-inline RO.o; case: ((r \in RO.m){1}).
-+ conseq (: _ ==> ={b} /\ Game1.r{2} \in Log.qs{2})=> //=.
-  + by move=> /> &1 &2 _ _ rR _ _ _ _ _ h /h [] -> //.
-  by auto=> /> &2 <- ->.
-rcondt{1} 3; 1:by auto.
-auto=> /> &2 log_is_dom r_notin_m y _; rewrite !get_set_sameE oget_some /=.
-split.
-+ by move=> _; rewrite eq_exceptP /pred1=> x; rewrite get_setE eq_sym=> ->.
-by move=> _ rR aL mL aR qsR mR h /h [] ->.
++ by apply A_guess_ll.
++ by proc; inline *; auto => /> &1 &2 hb; smt (eq_except_set_eq get_setE).
++ by move=> *; islossless.
++ by move=> /=; proc; call (_: true); 1: islossless; auto => />.
+inline Hash.hash; auto => /=.
+call (_: ={glob Hash} /\ (forall x, x \in Hash.qs{2} = x \in RO.m{2})).
++ by proc; inline *;auto => />; smt (get_setE).
+by inline *;auto => />; smt (mem_empty eq_except_setl get_setE).
 qed.
 
 (* Step 2: replace h ^ m with h in the challenge encryption            *)
@@ -319,32 +289,28 @@ local module Game2 = {
 
   proc main() = {
     var pk, sk, m0, m1, b, h, c, b';
-                Log(RO).init();
+                Hash.init();
     (pk,sk)  <$ dkeys;
-    (m0,m1)  <@ A(Log(RO)).a1(pk);
-    b        <$ {0,1};
-
+    (m0,m1)  <@ A(Hash).choose(pk);
     r        <$ drand;
     h        <$ dptxt;
     c        <- ((f pk r),h);
-
-    b'       <@ A(Log(RO)).a2(c);
+    b'       <@ A(Hash).guess(c);
+    b        <$ {0,1};
     return b' = b;
   }
 }.
 
 local equiv eq_Game1_Game2: Game1.main ~ Game2.main:
-  ={glob A} ==> ={glob Log, res} /\ Game1.r{1} = Game2.r{2}.
+  ={glob A} ==> ={glob Hash, res} /\ Game1.r{1} = Game2.r{2}.
 proof.
-proc.
-call (: ={glob Log, glob RO}); 1: by sim.
-wp; rnd (fun x=> x +^ (b?m0:m1){2}).
-auto; call (: ={glob Log, glob RO}); 1: by sim.
+proc. swap{2} -4.
+call (: ={glob Hash}); 1: by sim.
+wp; rnd (fun x=> x +^ (b?m1:m0){2}).
+auto; call (: ={glob Hash}); 1: by sim.
 inline *; auto=> /> _ _ rR b _ rL _; split=> [|_].
 + by move=> hR _; rewrite addpK.
-split=> [|_].
-+ by move=> hR _; exact/dptxt_funi.
-by move=> hL _; rewrite dptxt_fu /= addpK.
+by move=> hL _; rewrite addpK.
 qed.
 
 local lemma pr_Game1_Game2 &m:
@@ -352,309 +318,148 @@ local lemma pr_Game1_Game2 &m:
 proof. by byequiv eq_Game1_Game2. qed.
 
 local lemma pr_bad_Game1_Game2 &m:
-    Pr[Game1.main() @ &m: Game1.r \in Log.qs]
-  = Pr[Game2.main() @ &m: Game2.r \in Log.qs].
+    Pr[Game1.main() @ &m: Game1.r \in Hash.qs]
+  = Pr[Game2.main() @ &m: Game2.r \in Hash.qs].
 proof. by byequiv eq_Game1_Game2. qed.
 
-local lemma pr_Game2 &m: Pr[Game2.main() @ &m: res] = 1%r / 2%r.
+local lemma pr_Game2 &m: Pr[Game2.main() @ &m: res] <= 1%r / 2%r.
 proof.
 byphoare=> //=; proc.
-swap 4 4.
-wp; rnd (pred1 b')=> //=.
-inline *; call (_: true).
-+ exact A_a2_ll. (* adversary *)
-+ by proc; call (RO_o_ll dptxt_ll); auto. (* oracle *)
-auto; call (_: true).
-+ exact A_a1_ll. (* adversary *)
-+ by proc; call (RO_o_ll dptxt_ll); auto. (* oracle *)
-auto=> />; rewrite dkeys_ll drand_ll dptxt_ll /predT /=.
-by move=> _ _ _ _ _ _ r; rewrite dbool1E pred1E.
+by rnd (pred1 b'); conseq (: true) => // /> *; rewrite dbool1E.
 qed.
 
 (* Step 3: The reduction step -- if A queries the RO with the randomness *)
 (*     used to encrypt the challenge, then I(A) inverts the OW challenge *)
-(* We need a version of the one-way game where the challenge is a global *)
-local module OWr (I : Inverter) = {
-  var x : rand
-
-  proc main() : bool = {
-    var x', pk, sk;
-
-    (pk,sk) <$ dkeys;
-    x       <$ drand;
-    x'      <@ I.invert(pk,f pk x);
-    return (x = x');
-  }
-}.
-
-(* We can easily prove that it is strictly equivalent to OW              *)
-local lemma OW_OWr &m (I <: Inverter {-OWr}):
-  Pr[OW(I).main() @ &m: res]
-  = Pr[OWr(I).main() @ &m: res].
-proof. by byequiv=> //=; sim. qed.
 
 local lemma pr_Game2_OW &m:
-  Pr[Game2.main() @ &m: Game2.r \in Log.qs]
+  Pr[Game2.main() @ &m: Game2.r \in Hash.qs]
   <= Pr[OW(I(A)).main() @ &m: res].
 proof.
-rewrite (OW_OWr &m (I(A))). (* Note: we proved it forall (abstract) I    *)
-byequiv => //=; proc; inline *; wp.
-conseq
-  (_ : _ ==>
-       support dkeys (pk0{2}, sk{2}) /\
-       Game2.r{1} = OWr.x{2} /\ Log.qs{1} = Log.qs{2} /\
-       y{2} = f pk0{2} Game2.r{1}).
-+ move=> /> qs x pk sk vk x_in_qs; pose P := fun p => f _ p = _.
-  have h := nth_find witness P qs _.
-  + by rewrite hasP; exists x.
-  apply/(fI pk).
-  + by exists sk.
-  by rewrite h.
-(* rest of proof *)
-call (: ={glob Log, glob RO}); 1: by sim.
-swap{1} 6 -2.
-auto; call (: ={glob Log, glob RO}); 1: by sim.
-by auto=> /> [pk sk] ->.
+byequiv => //=; proc; inline *.
+swap{1} 5 -1.
+rnd{1}; wp.
+call (_: ={glob Hash}); 1: by sim.
+auto.
+call (_: ={glob Hash}); 1: by sim.
+auto => /> -[pk sk] hkeys r _ h _ qs _ _ hin.
+pose P := fun p => f _ p = _.
+apply/(fI pk); 1: by exists sk.
+have <- // := (nth_find witness P qs _).
+by rewrite hasP; exists r.
 qed.
 
 lemma Reduction &m:
-  Pr[BR93_CPA(A).main() @ &m : res] - 1%r/2%r
+  Pr[CPA(BR93(Hash), A(Hash)).main() @ &m : res] - 1%r/2%r
   <= Pr[OW(I(A)).main() @ &m: res].
 proof.
 smt(pr_Game0_Game1 pr_Game1_Game2 pr_bad_Game1_Game2 pr_Game2 pr_Game2_OW).
 qed.
+
 end section.
-end BR93.
 
-(* We now consider a concrete instance:                                 *)
-(*   - plaintexts are bitstrings of length k > 0                        *)
-(*   - nonces are bitstrings of length l > 0                            *)
-(*   - ciphertexts are bitstrings of length n = k + l                   *)
-
-(* Plaintexts                                                           *)
-op k : { int | 0 < k } as gt0_k.
-
-clone import BitWord as Plaintext with
-  op n <- k
-proof gt0_n by exact/gt0_k
-rename
-  "word" as "ptxt"
-  "dunifin" as "dptxt".
-import DWord.
-
-(* Nonces                                                               *)
-op l : { int | 0 < l } as gt0_l.
-
-clone import BitWord as Randomness with
-  op n <- l
-proof gt0_n by exact/gt0_l
-rename
-  "word" as "rand"
-  "dunifin" as "drand".
-import DWord.
-
-(* Ciphertexts                                                          *)
-op n = l + k.
-lemma gt0_n: 0 < n by smt(gt0_k gt0_l).
-
-clone import BitWord as Ciphertext with
-  op n <- n
-proof gt0_n by exact/Self.gt0_n
-rename "word" as "ctxt".
-
-(* Parsing and Formatting                                               *)
-op (||) (r:rand) (p:ptxt) : ctxt = mkctxt ((ofrand r) ++ (ofptxt p)).
-op parse (c:ctxt): rand * ptxt =
-  (mkrand (take l (ofctxt c)),mkptxt (drop l (ofctxt c))).
-
-lemma parseK r p: parse (r || p) = (r,p).
-proof.
-rewrite /parse /(||) ofctxtK 1:size_cat 1:size_rand 1:size_ptxt //=.
-by rewrite take_cat drop_cat size_rand take0 drop0 cats0 /= mkrandK mkptxtK.
-qed.
-
-lemma formatI (r : rand) (p : ptxt) r' p':
-  (r || p) = (r' || p') => (r,p) = (r',p').
-proof. by move=> h; rewrite -(@parseK r p) -(@parseK r' p') h. qed.
-
-(* A set `pkey * skey` of keypairs, equipped with                       *)
-(*                         a lossless, full, uniform distribution dkeys *)
-type pkey, skey.
-op dkeys: { (pkey * skey) distr |    is_lossless dkeys
-                                  /\ is_funiform dkeys } as dkeys_llfuni.
-
-(* A family `f` of trapdoor permutations over `rand`,                   *)
-(*        indexed by `pkey`, with inverse family `fi` indexed by `skey` *)
-op f : pkey -> rand -> rand.
-op fi: skey -> rand -> rand.
-axiom fK pk sk x: (pk,sk) \in dkeys => fi sk (f pk x) = x.
-
-(* Random Oracle                                                        *)
-clone import ROM.Lazy as H with
-  type from      <- rand,
-  type to        <- ptxt,
-  op   dsample _ <- dptxt.
-
-(* A Definition for OWTP Security                                       *)
-module type Inverter = {
-  proc invert(pk:pkey, x:rand): rand
+type adv_cost = {
+  cchoose : int; (* cost *)
+  ochoose : int; (* number of call to o *)
+  cguess  : int; (* cost *)
+  oguess  : int; (* number of call to o *)
 }.
 
-module Exp_OW (I : Inverter) = {
-  proc main(): bool = {
-    var pk, sk, x, x';
-
-    (pk,sk) <$ dkeys;
-    x       <$ drand;
-    x'      <@ I.invert(pk,f pk x);
-    return (x = x');
-  }
-}.
-
-(* A Definition for CPA Security                                        *)
-module type Scheme (RO : Oracle) = {
-  proc keygen(): (pkey * skey)
-  proc enc(pk:pkey, m:ptxt): ctxt
-}.
-
-module type Adv (ARO : ARO)  = {
-  proc a1(p:pkey): (ptxt * ptxt)
-  proc a2(c:ctxt): bool
-}.
-
-module CPA (O : Oracle) (S:Scheme) (A:Adv) = {
-  proc main(): bool = {
-    var pk, sk, m0, m1, c, b, b';
-
-               O.init();
-    (pk,sk) <@ S(O).keygen();
-    (m0,m1) <@ A(O).a1(pk);
-    b       <$ {0,1};
-    c       <@ S(O).enc(pk,b?m0:m1);
-    b'      <@ A(O).a2(c);
-    return b' = b;
-  }
-}.
-
-(* And a definition for the concrete Bellare-Rogaway Scheme             *)
-module (BR : Scheme) (H : Oracle) = {
-  proc keygen():(pkey * skey) = {
-    var pk, sk;
-
-    (pk,sk) <$ dkeys;
-    return (pk,sk);
-  }
-
-  proc enc(pk:pkey, m:ptxt): ctxt = {
-    var h, r;
-
-    r <$ drand;
-    h <@ H.o(r);
-    return ((f pk r) || m +^ h);
-  }
-
-  proc dec(sk:skey, c:ctxt): ptxt = {
-    var r, p, h;
-
-    (r,p) <- parse c;
-    r     <- fi sk r;
-    h     <@ H.o(r);
-    return p +^ h;
-  }
-}.
-
-(* And our inverter                                                     *)
-module I (A:Adv) (H : Oracle) = {
-  var qs : rand list
-
-  module QRO = {
-    proc o(x:rand) = {
-      var r;
-
-      qs <- x::qs;
-      r  <@ H.o(x);
-      return r;
-    }
-  }
-
+module Ifind(A:Adv) = {
   proc invert(pk:pkey,y:rand): rand = {
-    var x, m0, m1, h, b;
+    var m0, m1, h, b, r, x;
 
-    qs      <- [];
-               H.init();
-    (m0,m1) <@ A(QRO).a1(pk);
+               Hash.init();
+    (m0,m1) <@ A(Hash).choose(pk);
     h       <$ dptxt;
-    b       <@ A(QRO).a2(y || h);
-    x       <- nth witness qs (find (fun p => f pk p = y) qs);
-
+    b       <@ A(Hash).guess(y,h);
+    x <- witness; 
+    while (Hash.qs <> []){
+      r <- head witness Hash.qs; 
+      if (f pk r = y) {
+        x <- r; Hash.qs <- [];
+      } else {
+        Hash.qs <- drop 1 Hash.qs;
+      }
+    }
     return x;
   }
 }.
 
-(* We will need to turn a concrete CPA adversary into an abstract one.  *)
-(*      We do not need to do it for the inverter as the types coincide. *)
-module A_CPA (A : Adv) (H : ARO) = {
-  proc a1 = A(H).a1
-
-  proc a2(c:rand * ptxt): bool = {
-    var b;
-
-    b <@ A(H).a2(c.`1 || c.`2);
-    return b;
-  }
-}.
-
-section.
-declare module A : Adv { -RO, -I }.
-
-axiom A_a1_ll (O <: ARO {-A}): islossless O.o => islossless A(O).a1.
-axiom A_a2_ll (O <: ARO {-A}): islossless O.o => islossless A(O).a2.
-
-local clone import BR93 as Instance with
-  type pkey  <- pkey,
-  type skey  <- skey,
-  op   dkeys <- dkeys,
-  op   f     <- f,
-  op   fi    <- fi,
-  type ptxt  <- ptxt,
-  op   (+^)  <- Plaintext.(+^),
-  op   dptxt <- dptxt,
-  type rand  <- rand,
-  op   drand <- drand
-proof addA, addC, addKp, dptxt_llfuuni, drand_lluni, dkeys_llfuni, fK.
-realize addA          by move=> p1 p2 p3; algebra.
-realize addC          by move=> p1 p2; algebra.
-realize addKp         by move=> p1 p2; algebra.
-realize dptxt_llfuuni by smt(@Plaintext.DWord).
-realize drand_lluni   by smt(@Randomness.DWord).
-realize dkeys_llfuni  by exact/dkeys_llfuni.
-realize fK            by exact/fK.
-
-lemma Reduction &m:
-     Pr[CPA(RO, BR, A).main() @ &m : res] - 1%r / 2%r
-  <= Pr[Exp_OW(Self.I(A, RO)).main() @ &m : res].
+lemma ex_Reduction (cA:adv_cost) (A<:Adv [choose : `{cA.`cchoose, #ARO.o : cA.`ochoose},
+                                          guess  : `{cA.`cguess,  #ARO.o : cA.`oguess}] {-Hash}) &m:
+  (0 <= cA.`cchoose /\ 0 <= cA.`ochoose /\ 0 <= cA.`cguess /\ 0 <= cA.`oguess) =>
+  (forall (O <: ARO{-A}), islossless O.o => islossless A(O).guess) =>
+  let qH = cA.`ochoose + cA.`oguess in
+  let cB = 
+    4 + (4 + cf + ceqrand) * (cA.`ochoose + cA.`oguess) + cdptxt + 
+    (3 + cdptxt + cget qH + cset qH + cin qH) * (cA.`ochoose + cA.`oguess) +
+    cA.`cguess + cA.`cchoose in
+  exists (B <: Inverter [invert : `{cB} ]),
+    Pr[CPA(BR93(Hash), A(Hash)).main() @ &m : res] - 1%r/2%r <= Pr[OW(B).main() @ &m: res].  
 proof.
-have <-:   Pr[BR93_CPA(A_CPA(A)).main() @ &m: res]
-         = Pr[CPA(RO,BR,A).main() @ &m: res].
-+ byequiv=> //=; proc.
-  inline A_CPA(A,Log(H.RO)).a2.
-  wp; call (: H.RO.m{1} = RO.m{2}).
-  + by proc; inline *; auto.
-  inline BR93(H.RO).enc BR(RO).enc H.RO.o RO.o; auto.
-  call (: H.RO.m{1} = RO.m{2}).
-  + by proc; inline *; auto.
-  inline *; auto=> /> [pk sk] _ [m0 m1] c b _ r _ h _ /=.
-  by rewrite addC /= addC.
-have <-:   Pr[OW_rand.OW(I(A_CPA(A))).main() @ &m: res]
-         = Pr[Exp_OW(Self.I(A,RO)).main() @ &m: res].
-+ byequiv=> //=; proc.
-  inline *; auto; call (: H.RO.m{1} = RO.m{2} /\ ={qs}(Log,Self.I)).
-  + by sim.
-  auto; call (: H.RO.m{1} = RO.m{2} /\ ={qs}(Log,Self.I)).
-  + by sim.
-  by auto.
-apply/(Reduction (A_CPA(A)) _ _ &m).
-+ by move=> O O_o_ll; exact/(A_a1_ll O O_o_ll).
-by move=> O O_o_ll; proc; call (A_a2_ll O O_o_ll).
+  move=> cA_pos A_choose_ll qH.
+  exists (Ifind(A)); split.  
+  (* Proof of the complexity *)
+  + proc.
+    seq 5 : (size Hash.qs <= cA.`ochoose + cA.`oguess) time [(4 + cf + ceqrand) * (cA.`ochoose + cA.`oguess) + 2].
+    + wp.
+      call (_: bounded RO.m (size Hash.qs);
+           (Hash.o : size Hash.qs- cA.`ochoose) 
+           time
+           [(Hash.o : [fun _ => 3 + cdptxt + cget qH + cset qH + cin qH])]).
+      + move=> zo hzo; proc; inline *.
+        wp : (bounded RO.m qH).
+        by auto => &hr />; rewrite dptxt_ll /=; smt (cset_pos bounded_set).
+      auto; call (_: bounded RO.m (size Hash.qs);
+           (Hash.o : size Hash.qs)
+           time [(Hash.o : [fun _ => 3 + cdptxt + cget qH + cset qH + cin qH])]).
+      + move=> zo hzo; proc; inline *.
+        wp : (bounded RO.m qH).
+        by auto => &hr />; rewrite dptxt_ll /=; smt(cset_pos bounded_set).
+      inline *; auto => />; split => *.
+      + smt (bounded_empty dptxt_ll size_ge0 size_eq0).
+      rewrite !bigi_constz /= /#.
+    while (true) (size Hash.qs) (cA.`ochoose + cA.`oguess) time [fun _ => 2 + cf + ceqrand].
+    + move => z /=; auto => &hr H /=; smt (size_ge0).
+    + move => &hr; smt (size_ge0 size_eq0). 
+    by auto => /> &hr; rewrite bigi_constz /#.
+  (* Proof of the bound *)
+  have := Reduction A A_choose_ll &m.
+  have -> //: Pr[OW(I(A)).main() @ &m : res] = Pr[OW(Ifind(A)).main() @ &m : res].
+  + byequiv => //; proc; inline *; wp.
+  while{2}  
+   (if Hash.qs{2} = [] then 
+       x0{2} = nth witness Hash.qs{1} (find (fun r => f pk0{2} r = y{2}) Hash.qs{1})
+    else 
+     exists i, x0{2} = witness /\ 0 <= i < size Hash.qs{1} /\ Hash.qs{2} = drop i Hash.qs{1} /\ 
+               !has (fun r => f pk0{2} r = y{2}) (take i Hash.qs{1}))
+   (size Hash.qs{2}).  
+  + move=> &1 z; auto => &2 />.
+    case: (Hash.qs{2}) => //= hd qs0 [i />] h0i hi hdr hhas.
+    have heq : Hash.qs{1} = take i Hash.qs{1} ++ hd :: qs0.
+    + by rewrite hdr cat_take_drop.
+    rewrite heq; move: hhas; (pose tk := take i Hash.qs{1}) => hhas.
+    have heq1 : 
+     nth witness (tk ++ hd :: qs0) (find (fun (p0 : rand) => f pk0{2} p0 = y{2}) (tk ++ hd :: qs0)) =
+     nth witness (hd :: qs0) (find (fun (p0 : rand) => f pk0{2} p0 = y{2}) (hd :: qs0)).
+    + by rewrite find_cat hhas /= nth_cat; smt (find_ge0).
+    split. 
+    + move=> heq2;rewrite heq2 heq1 /= heq2 /=; smt (size_ge0).  
+    rewrite heq1 drop0 => hy; split;2:smt().
+    split.
+    + by move=> />;rewrite hy.
+    move=> hqs; exists (i + 1).
+    rewrite size_cat /= -cat_rcons.
+    have -> : i + 1 = size (rcons tk hd).
+    + by rewrite size_rcons size_take // hi.
+    rewrite drop_size_cat // take_size_cat // size_rcons -cats1 has_cat /=.
+    smt (size_ge0).
+  wp.
+  conseq (: ={Hash.qs, pk0, x, y}).
+  + move=> /> *; split; last by smt (size_eq0 size_ge0).
+    by move=> *; exists 0; rewrite drop0 take0 /=; smt (size_eq0 size_ge0).
+  by sim.
 qed.
-end section.
+
+end BR93.
+
