examples/hashed_elgamal_generic.ec
@@ -86,6 +86,9 @@ clone import ROM.Lazy as ROL with
   op dsample <- fun (x:group), dbits
 proof * by exact/dbits_ll.
 
+clone import FMapCost as FMC with
+  type from  <- group.
+
 (* Adversary Definitions *)
 module type Adversary (O:ARO) = {
   proc choose(pk:pkey): ptxt * ptxt
@@ -103,92 +106,8 @@ module H = {
 (* The initial scheme *)
 module S = Hashed_ElGamal(H).
 
-(*
-(* The reduction *)
-module SCDH_from_CPA(A:Adversary,O:Oracle): SCDHT.Adversary = {
-  module BA = A(Bound(O))
-
-  proc solve(gx:group, gy:group): group fset = {
-    var m0, m1, h, b';
-
-    H.init();
-    (m0,m1)  <@ BA.choose(gx);
-    h        <$ dbits;
-    b'       <@ BA.guess(gy, h);
-    return Log.qs;
-  }
-}.
-*)
 (* We want to bound the probability of A winning CPA(Bounder(A,RO),S) in terms of
    the probability of B = CDH_from_CPA(SCDH_from_CPA(A,RO)) winning CDH(B) *)
-
-(* FIXME: move this *)
-schema cost_eqnil ['a] `{P} {l:'a list} : cost [P: l = []] = cost [P:l] + 1.
-hint simplify cost_eqnil.
-
-schema cost_oget ['a] `{P} {o: 'a option} : 
-  cost [P : oget o] = cost [P:o] + 1.
-hint simplify cost_oget.
-
-schema cost_empty ['a 'b] `{P} :
-  cost [P: empty<:'a, 'b>] = 1.
-hint simplify cost_empty.
-
-op bounded ['from 'to] (m : ('from, 'to)fmap) (size:int) = 
-   card (fdom m) <= size.
-
-lemma bounded_set ['from 'to] (m : ('from, 'to)fmap) (size:int) x e : 
-  bounded m size => bounded (m.[x<-e]) (size + 1).
-proof. by rewrite /bounded fdom_set fcardU fcard1; smt (fcard_ge0). qed.
-
-lemma bounded_empty ['from 'to] : bounded empty<:'from, 'to> 0.
-proof. by rewrite /bounded fdom0 fcards0. qed.
-
-abstract theory FMapCost.
-  type from.
-  type to.
-
-  op cget : int -> int.
-  op cset : int -> int.
-  op cin  : int -> int.
-
-  axiom cget_pos (x:int) : 0 <= cget x.
-  axiom cset_pos (x:int) : 0 <= cset x.
-  axiom cin_pos (x:int) : 0 <= cin x.
-
- 
-  (* Fixme, this need to be generalized in the schema *)
-  (* maximal size of the map *)
-  op max_size : int.
-
-  schema cost_get_P ['a 'b] `{P} {m:('a, 'b) fmap, x:'a} :
-    cost [P /\ bounded m max_size : m.[x]] = cost[P:m] + cost[P:x] + cget max_size.
-
-  schema cost_set_P ['a 'b] `{P} {m:('a, 'b) fmap, x:'a, e:'b} :
-    cost [P /\ bounded m max_size : m.[x<-e]] = cost[P:m] + cost[P:x] + cost[P:e] + cset max_size.
-
-  schema cost_in_P ['a 'b] `{P} {m:('a, 'b) fmap, x:'a} :
-    cost [P /\ bounded m max_size: x \in m] = cost[P:m] + cost[P:x] + cin max_size.
-
-  hint simplify cost_get_P, cost_set_P, cost_in_P.
-
-  schema cost_get ['a 'b] {m:('a, 'b) fmap, x:'a} :
-    cost [bounded m max_size : m.[x]] = cost[true:m] + cost[true:x] + cget max_size.
-
-  schema cost_set ['a 'b] {m:('a, 'b) fmap, x:'a, e:'b} :
-    cost [bounded m max_size : m.[x<-e]] = cost[true:m] + cost[true:x] + cost[true:e] + cset max_size.
-
-  schema cost_in ['a 'b] {m:('a, 'b) fmap, x:'a} :
-    cost [bounded m max_size: x \in m] = cost[true:m] + cost[true:x] + cin max_size.
-
-  hint simplify cost_get, cost_set, cost_in.
-
-end FMapCost.
-
-clone import FMapCost as FMC with
-  type from  <- group,
-  type to    <- bits,
-  op max_size <- qH.
 
 section.
 
@@ -263,15 +182,13 @@ section.
     }
   }. 
 
-  op foo : int.
-
   local lemma cost_ALCDH : 
     choare [ALCDH.solve : true ==> 0 < size res <= cA.`ochoose + cA.`oguess] 
     time [6 + cunifin + (3 + cunifin + cget qH + cset qH + cin qH) * (cA.`oguess + cA.`ochoose) + cA.`cguess + cA.`cchoose].
   proof.
     proc; wp.
     call (_: bounded RO.m (size H.qs);
-           (H.o : size H.qs- cA.`ochoose)
+           (H.o : size H.qs- cA.`ochoose) 
            time
            [(H.o : [fun _ => 3 + cunifin + cget qH + cset qH + cin qH])]).
     + move=> zo hzo; proc; inline *.
